process/subject_reduction.v
@@ -574,6 +574,108 @@ Proof.
     subst. exists m. easy.
   apply multiC_refl.
   
+  (* R-COMM *)
+  inversion H1. subst.
+  - inversion H5. subst. clear H5. inversion H8. subst. clear H8. 
+    inversion H9. subst. clear H9.
+    destruct H6 as (T,(Ha,(Hb,Hc))). destruct H7 as (T1,(Hd,(He,Hf))).
+    - specialize(_a23_a q xs (p_recv q xs) nil nil T Hb (eq_refl (p_recv q xs))); intros. 
+      destruct H5 as (STT,(Hg,(Hh,(Hi,Hj)))).
+    - specialize(_a23_bf p l e Q (p_send p l e Q) nil nil T1 He (eq_refl (p_send p l e Q))); intros.
+      destruct H5 as (S,(T',(Hk,(Hl,Hm)))).
+    
+    specialize(_3_19_h q p l); intros.
+    specialize(subtype_recv T q STT Hh); intros. destruct H6. subst.
+    specialize(subtype_send T1 p (extendLis l (Some (S, T'))) Hm); intros. destruct H6. subst.
+    rename x into LQ. rename x0 into LP.
+    specialize(H5 G LP LQ S T').
+    specialize(_3_21_helper l xs STT y H Hi); intros. destruct H6. destruct H6. destruct H6.
+    specialize(H5 STT (x, x0)). 
+    assert(exists G' : gtt, gttstepC G G' q p l).
+    apply H5; try easy. destruct H8. subst. rename x1 into G'. 
+    assert(multiC G G').
+    specialize(multiC_step G G' G' q p l); intros. apply H9; try easy. constructor.
+    exists G'. split; try easy.
+    specialize(wfgC_after_step G G' q p l H2 H8); intros. 
+    assert(wfgC G').
+    intros. apply H10.
+    unfold projectableA. intros.
+    specialize(decidable_isgPartsC G pt H2); intros. unfold Decidable.decidable in H11.
+    destruct H11.
+    specialize(H3 pt H11).
+    - unfold InT in H3. simpl in H3.
+      - destruct H3. subst. exists (ltt_recv q LQ). easy.
+      - destruct H3. subst. exists (ltt_send p LP). easy.
+      - easy.
+    - unfold not in H11. exists ltt_end. pfold. constructor; try easy.
+    constructor; try easy.
+    - intros.
+      apply H3; try easy.
+      - specialize(part_after_step G G' q p pt l LP LQ); intros. 
+        apply H13; try easy.
+    specialize(projection_step_label G G' q p l LP LQ); intros.
+    assert(exists (LS LS' : sort) (LT LT' : ltt), onth l LP = Some (LS, LT) /\ onth l LQ = Some (LS', LT')).
+    apply H12; try easy.
+    destruct H13 as (SL,(SL',(TL,(TL',(H22,H23))))).
+    
+    specialize(_a_29_s G q p LP LQ SL TL SL' TL' l H2 Hd H22 Ha H23); intros.
+    destruct H13 as (Gl,(ctxG,(SI,(Sn,(Hta,(Htb,(Htc,(Htd,(Hte,(Htf,Htg)))))))))).
+    specialize(_3_21_helper_1 H23 H6 Hh); intros.
+    specialize(_3_21_helper_2 Hm H22); intros. 
+    constructor. constructor.
+    - specialize(_3_19_2_helper q p l G G' LP LQ SL TL SL' TL'); intros.
+      assert(projectionC G' p TL'). apply H15; try easy. clear H15. 
+      exists TL'. split; try easy.
+      split.
+      apply _a24 with (S := x); try easy.
+      - apply tc_sub with (t := x0); try easy.
+        specialize(typable_implies_wfC Hb); intros.
+        specialize(wfC_recv H15 H23); try easy.
+      - apply sc_sub with (s := S); try easy.
+        apply expr_typ_step with (e := e); try easy.
+        apply sstrans with (s2 := SL'); try easy.
+        apply sstrans with (s2 := Sn); try easy. 
+        apply sstrans with (s2 := SL); try easy.
+      - specialize(guardP_cont_recv_n l xs y q Hc H); intros.
+        specialize(guardP_subst_expr y (e_val v) 0 0); intros. apply H17; try easy.
+    - constructor.
+      specialize(_3_19_1_helper q p l G G' LP LQ SL TL SL' TL'); intros.
+      assert(projectionC G' q TL). apply H15; try easy. clear H15.
+      exists TL. split; try easy. split.
+      - apply tc_sub with (t := T'); try easy.
+        specialize(typable_implies_wfC He); intros.
+        specialize(wfC_send H15 H22); try easy.
+      - intros. specialize(Hf (Nat.succ n)). destruct Hf. inversion H15.
+        subst. exists x1. easy.
+
+  (* T-COND *)
+  inversion H0. subst. inversion H4. subst. clear H4.
+  destruct H6. destruct H4. destruct H5 as (H5, Ha).
+  specialize(_a23_c (p_ite e P Q) e P Q x nil nil H5 (eq_refl (p_ite e P Q))); intros.
+  destruct H6. destruct H6. destruct H6. destruct H7. destruct H8. destruct H9. 
+  exists G. split.
+  apply t_sess; try easy. constructor. exists x.
+  split; try easy. split.
+  apply tc_sub with (t := x0); try easy.
+  specialize(typable_implies_wfC H5); try easy.
+  - intros. specialize(Ha n). destruct Ha. inversion H11. subst. exists 0. constructor.
+    subst. exists m. easy.
+  apply multiC_refl.
+  
+  (* F-COND *)
+  inversion H0. subst. inversion H4. subst. clear H4.
+  destruct H6. destruct H4. destruct H5 as (H5, Ha).
+  specialize(_a23_c (p_ite e P Q) e P Q x nil nil H5 (eq_refl (p_ite e P Q))); intros.
+  destruct H6. destruct H6. destruct H6. destruct H7. destruct H8. destruct H9. 
+  exists G. split.
+  apply t_sess; try easy. constructor. exists x.
+  split; try easy. split.
+  apply tc_sub with (t := x1); try easy.
+  specialize(typable_implies_wfC H5); try easy.
+  - intros. specialize(Ha n). destruct Ha. inversion H11. subst. exists 0. constructor.
+    subst. exists m. easy.
+  apply multiC_refl.
+  
   (* R-STRUCT *)
   specialize(_a22_2 M1 M1' G H2 H); intros.
   specialize(IHbetaP G H3); intros. destruct IHbetaP. exists x. 
